A12Kernel/Proofs.lean
@@ -39,6 +39,7 @@ import A12Kernel.Proofs.AddressedTimeConstructionFormalInput
 import A12Kernel.Proofs.TimeFromDateTimeComputation
 import A12Kernel.Proofs.AddressedTimeFromDateTime
 import A12Kernel.Proofs.AddressedTimeFromDateTimeFormalInput
+import A12Kernel.Proofs.AddressedDateRangeBoundPart
 import A12Kernel.Proofs.TimeInput
 import A12Kernel.Proofs.DateTimeInput
 import A12Kernel.Proofs.ValueAsDate
